\documentclass[12pt, letterpaper]{article}
\usepackage[utf8]{inputenc}
\usepackage{amsmath, amsfonts, amssymb}
\usepackage{geometry}
\usepackage{graphicx}
\usepackage{fancyhdr}
\usepackage{pgfplots}
\usepackage{float}
\usepackage{pgfplotstable}
\usepackage{booktabs} 
\usepackage{amsmath} % Add this line to include the amsmath package
\pgfplotsset{compat=1.18}

% Setup for homework style
\geometry{margin=1in}
\pagestyle{fancy}
\fancyhf{}
\lhead{APPM 2360: Differential Equations}
\rhead{Homework 3}
\cfoot{\thepage}

\title{Homework 3}
\author{Zachariah Galdston}
\date{9/12/2024}

\begin{document}

\maketitle

\section*{Problem 1}

\textbf{Problem Statement:} Determine weather Picard's Theorem can be used to show the existence of a unique solution in an open interval containing t = 0

\textbf{Solution:} Picards theorem sates that if $f(t,y)$ is continuous in some region $R$ defined by 
\[ \{(t,y) \,|\, a < t < b, c < y < d\} \] 

and $(t_0, y_0) \in \mathbb{R}$. Then there exists a postivie number $h$ such that the IVP
\[ y' = f(t,y), \quad y(t_0) = y_0\]
Has a solution in an open interval containing $(t_0 - h, t_0 + h)$. The solution is unique if $\frac{\partial f}{\partial y}$ is continuous in $R$

\subsection*{(a) $y' = ty^{\frac{4}{3}}, \quad y(0) = 0$}
\textbf{Problem Statement:} Determine weather Picard's Theorem can be used to show the existence of a unique solution in an open interval containing t = 0

\textbf{Solution:} We will start by determining the continutiy of the function $f(t) = ty^{\frac{4}{3}}$ by finding the partial derivative of $f$ with respect to $y$ \\

Existence: $f(t) = ty^{\frac{4}{3}}$ is continuous for all $t$ and $y$ in the region $R$. Therefore, Picard's Theorem can be used to show the existence of a  solution in an open interval containing $t = 0$. \\

Uniqueness: We will find the partial derivative of $f$ with respect to $y$

\begin{align*}
\frac{\partial f}{\partial y} &= \frac{4}{3}ty^{\frac{1}{3}}
\end{align*}

Since $\frac{\partial f}{\partial y}$ is continuous for all $t$ and $y$ in the region $R$Picard's Theorem can be used to show the existence of a unique solution in an open interval containing $t = 0$.

\subsection*{(b) $y' = ty^{1/3}, \quad y(0) = 0$}
\textbf{Problem Statement:} Determine weather Picard's Theorem can be used to show the existence of a unique solution in an open interval containing t = 0

\textbf{Solution:} We will start by determining the continutiy of the function $f(t) = ty^{\frac{1}{3}}$ 
\paragraph*{}
Existence: $f(t) = ty^{\frac{1}{3}}$ is continuous for all $t$ and $y$ in the region $R$ Therefore, Picard's Theorem can be used to show the existence of a  solution in an open interval containing $t = 0$. \\

Uniqueness: We will find the partial derivative of $f$ with respect to $y$ \\
\begin{align*}
\frac{\partial f}{\partial y} &= \frac{1}{3}ty^{-\frac{2}{3}}
\end{align*}

Since $\frac{\partial f}{\partial y}$ is not continuous ($\frac{1}{\sqrt[3]{0}^2} = DNE$ ) for all $t$ and $y$ in the region $R$ , Picard's Theorem cannot be used to show the existence of a unique solution in an open interval containing $t = 0$.

\subsection*{(c) $y' = ty^{\frac{1}{3}}, \quad y(0) = 1$}
\textbf{Problem Statement:} Determine weather Picard's Theorem can be used to show the existence of a unique solution in an open interval containing t = 0

\textbf{Solution:} We will start by determining the continutiy of the function $f(t) = ty^{\frac{1}{3}}$

Existence: $f(t) = ty^{\frac{1}{3}}$ is continuous for all $t$ and $y$ in the region $R$. Therefore, Picard's Theorem can be used to show the existence of a  solution in an open interval containing $t = 0$. \\

Uniqueness: We will find  the partial derivative of $f$ with respect to $y$ \\
\begin{align*}
\frac{\partial f}{\partial y} &= \frac{1}{3}ty^{-\frac{2}{3}}
\end{align*}

Since $\frac{\partial f}{\partial y}$ is continuous for all $t$ and $y$ in the region $R$, Picard's Theorem can be used to show the existence of a unique solution in an open interval containing $t = 0$.

\section*{Problem 2}

\textbf{Problem Statement:} Find the order, linearity, homogeneity, and the variablity of the coefficients of the following:

%I want to make a table for this problem, with the diff eqs a-e on the left and then the solutions on the right
\begin{table}[H]
    \centering
    \begin{tabular}{|c|c|c|c|c|c|}
        \hline
        \textbf{Problem} & \textbf{Diff Eq} & \textbf{Order} & \textbf{Linearity} & \textbf{Homogeneity} & \textbf{coefficients} \\
        \hline
        (a) & $y'' + 2y' + y = 0$ & 2 & Linear & Homogeneous & Constant \\
        \hline
        (b) & $\ddot x + 2\dot x + tx = \sin(t)$ & 2 & Linear & Non-Homogeneous & Variable \\
        \hline
        (c) & $\cos(y') + ty = 0$ & 1 & Non-Linear & Homogeneous & Variable \\
        \hline
        (d) & $y'' + ey' + \pi y = 0$ & 2 & Linear & Homogeneous & Constant \\
        \hline
        (e) & $y' + \frac{1}{1+t^2}y = 7$ & 1 & Linear & Non-Homogeneous & Variable \\
        \hline
    \end{tabular}
\end{table}

\section*{Problem 3}

\textbf{Problem Statement:} Which of the following operators are linear?

\textbf{Solution:} An operator is linear if it satisfies the following properties: 
\begin{align*}
    L(k\vec{\textbf{u}}) = kL(\vec{\textbf{u}}), \quad k \in \mathbb{R} \\
    L(\vec{\textbf{u}} + \vec{\textbf{w}}) = L(\vec{\textbf{u}}) + L(\vec{\textbf{w}})
\end{align*}

\subsection*{(a) $L(\vec{\textbf{y}}) = y' + 2ty$}
\textbf{Solution:} We will start by checking the first property
\begin{align*}
    L(k\vec{\textbf{u}}) &= kL(\vec{\textbf{u}}) \\
    L(ky) &= k(y' + 2ty) \\
    ky' + 2kty &= ky' + 2kty \\
    ky' + 2kty &= ky' + 2kty
\end{align*}

Now we will check the second property

\begin{align*}
    L(\vec{\textbf{u}} + \vec{\textbf{w}}) &= L(\vec{\textbf{u}}) + L(\vec{\textbf{w}}) \\
    L(y_1 + y_2) &= L(y_1) + L(y_2) \\
    y_1' + 2ty_1 + y_2' + 2ty_2 &= y_1' + 2ty_1 + y_2' + 2ty_2
\end{align*}

Since both properties are satisfied, the operator $L(\vec{\textbf{y}}) = y' + 2ty$ is linear

\subsection*{(b) $L(\vec{\textbf{y}}) = y'' + (1-y^2) + y$}
\textbf{Solution:} We will start by checking the first property
\begin{align*}
    L(k\vec{\textbf{u}}) &= kL(\vec{\textbf{u}}) \\
    L(ky) &= k(y'' + (1-y^2) + y) \\
    ky'' + (1-(ky)^2) + ky &\neq ky'' + k(1-y^2) + ky \\
\end{align*}

This does not satisfy the first property, so the operator $L(\vec{\textbf{y}}) = y'' + (1-y^2) + y$ is not linear. We will check the second property to be thorough.

\begin{align*}
    L(\vec{\textbf{u}} + \vec{\textbf{w}}) &= L(\vec{\textbf{u}}) + L(\vec{\textbf{w}}) \\
    L(y_1 + y_2) &= L(y_1) + L(y_2) \\
    y_1'' + (1-y_1^2) + y_1 + y_2'' + (1-y_2^2) + y_2 &\neq y_1'' + (1-y_1^2) + y_1 + y_2'' + (1-y_2^2) + y_2
\end{align*}

Since the second property is not satisfied, the operator $L(\vec{\textbf{y}}) = y'' + (1-y^2) + y$ is not linear.

\section*{Problem 4}
\textbf{Problem Statement:} Show that if $y_1(t)$ and $y_2(t)$ are solutions of $y' + p(t)y = 0$, then so are $y_1(t) + y_2(t)$ and $cy_1(t)$ for any constant $c$.

\textbf{Solution:} Assuming that $y_1(t)$ and $y_2(t)$ are solutions of $y' + p(t)y = 0$ and follow the properties of linear homogenoues ODEs. Thus,
\begin{align*}
    y_1' + p(t)y_1 &= 0 \\
    y_2' + p(t)y_2 &= 0
\end{align*}

Using the first property, we will show that $y_1(t) + y_2(t)$ is a solution of $y' + p(t)y = 0$
\begin{align*}
    (y_1 + y_2)' + p(t)(y_1 + y_2) &= 0 \\
    y_1' + y_2' + p(t)y_1 + p(t)y_2 &= 0 \\
    y_1' + p(t)y_1 + y_2' + p(t)y_2 &= 0 + 0 = 0 
\end{align*}

This proves that $y_1(t) + y_2(t)$ is a solution of $y' + p(t)y = 0$. 

Next we will show that $cy_1(t)$ is a solution of $y' + p(t)y = 0$
\begin{align*}
    (cy_1)' + p(t)(cy_1) &= 0 \\
    cy_1' + cp(t)y_1 &= 0 \\
    c(y_1' + p(t)y_1) &= c \cdot 0 = 0 
\end{align*}

This proves that $cy_1(t)$ is a solution of $y' + p(t)y = 0$.

\section*{Problem 5}
\textbf{Problem Statement:} Verify that the given functions $y_1(t)$ and $y_2(t)$ are solutions of the given differential equation. Then show that $c_1y_1(t) + c_2y_2(t)$ is also a solution for any real numbers $c_1$ and $c_2$.
\subsection*{(a) $y'' - y' + 6y = 0; \quad y_1(t) = e^{3t}, \quad y_2(t) = e^{-2t}$}

\textbf{Solution:} We will start by verifying that $y_1(t)$ and $y_2(t)$ are solutions of the given differential equation.
\begin{align*}
    y_1(t) &= e^{3t} \\
    y_1' &= 3e^{3t} \\
    y_1'' &= 9e^{3t} \\
    9e^{3t} - 3e^{3t} - 6e^{3t} &= 0
\end{align*}

Therefore, $y_1(t)$ is a solution of the given differential equation. Next we will verify that $y_2(t)$ is a solution
\begin{align*}
    y_2(t) &= e^{-2t} \\
    y_2' &= -2e^{-2t} \\
    y_2'' &= 4e^{-2t} \\
    4e^{-2t} + 2e^{-2t} - 6e^{-2t} &= 0
\end{align*}

Therefore, $y_2(t)$ is a solution of the given differential equation. Next we will show that $c_1y_1(t) + c_2y_2(t)$ is also a solution for any real numbers $c_1$ and $c_2$.

\begin{align*}
    c_1y_1(t) + c_2y_2(t) &= c_1e^{3t} + c_2e^{-2t} \\
\end{align*}

Now we will find the first and second derivatives of $c_1y_1(t) + c_2y_2(t)$

\begin{align*}
    (c_1y_1 + c_2y_2)' &= 3c_1e^{3t} - 2c_2e^{-2t} \\
    (c_1y_1 + c_2y_2)'' &= 9c_1e^{3t} + 4c_2e^{-2t} \\
\end{align*}

Pluging $c_1y_1 + c_2y_2$ into the differential equation,

\begin{align*}
    9c_1e^{3t} + 4c_2e^{-2t} - 3c_1e^{3t} + 2c_2e^{-2t} - 6c_1e^{3t} - 6c_2e^{-2t} &= 0 \\
    (9c_1 - 3c_1 - 6c_1)e^{3t} + (4c_2 + 2c_2 - 6c_2)e^{-2t} &= 0 \\
    0e^{3t} + 0e^{-2t} &= 0 \\
    0 &= 0
\end{align*}

Therefore, $c_1y_1(t) + c_2y_2(t)$ is a solution of the given differential equation.

\subsection*{(b) $y'' - 25y = 0; \quad y_1 = cosh(5t); y_2 = sinh(5t)$}

\textbf{Solution:} We will start by verifying that $y_1(t)$ and $y_2(t)$ are solutions of the given differential equation.

\begin{align*}
    y_1(t) &= cosh(5t) \\
    y_1' &= 5sinh(5t) \\
    y_1'' &= 25cosh(5t) \\
    25cosh(5t) - 25cosh(5t) &= 0
\end{align*}

Therefore, $y_1(t)$ is a solution of the given differential equation. Next we will verify that $y_2(t)$ is a solution

\begin{align*}
    y_2(t) &= sinh(5t) \\
    y_2' &= 5cosh(5t) \\
    y_2'' &= 25sinh(5t) \\
    25sinh(5t) - 25sinh(5t) &= 0
\end{align*}

Therefore, $y_2(t)$ is a solution of the given differential equation. Next we will show that $c_1y_1(t) + c_2y_2(t)$ is also a solution for any real numbers $c_1$ and $c_2$.

\begin{align*}
    c_1y_1(t) + c_2y_2(t) &= c_1cosh(5t) + c_2sinh(5t) \\
\end{align*}

Now we will find the first and second derivatives of $c_1y_1(t) + c_2y_2(t)$

\begin{align*}
    (c_1y_1 + c_2y_2)' &= 5c_1sinh(5t) + 5c_2cosh(5t) \\
    (c_1y_1 + c_2y_2)'' &= 25c_1cosh(5t) + 25c_2sinh(5t) \\
\end{align*}

Pluging $c_1y_1 + c_2y_2$ into the differential equation,

\begin{align*}
    25c_1cosh(5t) + 25c_2sinh(5t) - 25c_1cosh(5t) - 25c_2sinh(5t) &= 0
\end{align*}

Therefore, $c_1y_1(t) + c_2y_2(t)$ is a solution of the given differential equation.

\section*{Problem 6}
\textbf{Problem Statement:} Find the general solution to the non homogenoues ODE $y' + \frac{1}{t+1}y = 2$

\textbf{Solution:} We will solve using the superposition principal. $y_{G,NH} = y_{G,H} + y_{P,NH}$
\subsection*{(a)}
\textbf{Problem Satement:} Show that $y_p = \frac{t^2 + 2t}{t+1}$ is a particular solution to the Non-Homogeneous ODE $y' + \frac{1}{t+1}y = 2$

\textbf{Solution:} We will start by finding the derivative of $y_p$
\begin{align*}
y_p &= \frac{t^2 + 2t}{t+1} \\
y_p' &= \frac{(t+1)(2t+2) - (t^2 + 2t)}{(t+1)^2} \\
y_p' &= \frac{2t^2 + 2t + 2t + 2 - t^2 - 2t}{(t+1)^2} \\
y_p' &= \frac{t^2 + 4t + 2}{(t+1)^2}
\end{align*}

Now we will plug $y_p$ and $y_p'$ into the Non-Homogeneous ODE
\begin{align*}
y_p' + \frac{1}{t+1}y_p &= 2 \\
\frac{t^2 + 4t + 2}{(t+1)^2} + \frac{t^2 + 2t}{(t+1)^2} &= 2 \\
\frac{t^2 + 4t + 2 }{t^2 + 2t + 1} + \frac{t^2+2}{t^2 + 2t + 1} &= 2 \\
\frac{2t^2 + 4t + 2}{t^2 + 2t + 1} &= 2 \\
\frac{2(t^2 + 2t + 1)}{t^2 + 2t + 1} &= 2 \\
2 &= 2
\end{align*}

\subsection*{(b)}
\textbf{Problem Statement:} Find the general solution to the Non-Homogeneous ODE $y' + \frac{1}{t+1}y = 2$

\textbf{Solution:} We will use the superposition principal to find the general solution to the Non-Homogeneous ODE
\begin{align*}
y_{G,NH} &= y_{G,H} + y_{P,NH} \\
\end{align*}

Now we will the general solution to the Homogeneous ODE
\begin{align*}
y' + \frac{1}{t+1}y &= 0 \\
\frac{1}{y}dy = -\frac{1}{t+1}dt \\
\ln|y| = -\ln|t+1| + c \\
y = \frac{c}{t+1}
\end{align*}

Now we will find the general solution to the Non-Homogeneous ODE
\begin{align*}
y_{G,NH} &= \frac{c}{t+1} + \frac{t^2 + 2t}{t+1} \\
\end{align*}

\section*{Problem 7}
\textbf{Problem Statement:} Cosider the differential equation governing the current of an RL circuit $L\frac{dI}{dt} + RI = E(t)$ Suppose that $R = 100$ ohms, $L = 2.5$ henries, and the constant impressed voltage is $E(t) = E_0 = 110$ volts. Time $t$ is measured in seconds.

\subsection*{(a) If the initial curret is zero, find the current at any time}

\textbf{Solution:} We will start by finding the general solution to the Non-Homogeneous ODE

\begin{align*}
L\frac{dI}{dt} + RI &= E(t) \\
2.5\frac{dI}{dt} + 100I &= 110 \\
\frac{dI}{dt} + 40I &= 44
\end{align*}

We will use the integrating factor method.

\begin{align*}
\frac{dI}{dt} + 40I &= 44 \\
\mu &= e^{\int 40dt} \\
\mu &= e^{40t} \\
\end{align*}

Multiply the original equation by $\mu$

\begin{align*}
e^{40t}\frac{dI}{dt} + 40e^{40t}I &= 44e^{40t} \\
D[\mu I] &= 44 \mu \\
e^{40t}I &= \int 44e^{40t} \\
e^{40t}I &= \frac{44}{40} + ce^{40t} \\
I &= 1.1 + ce^{-40t}
\end{align*}

Solve the IVP $I(0) = 0$

\begin{align*}
0 &= 1.1 + c \\
c &= -1.1 \\
I &= 1.1 - 1.1e^{-40t}
\end{align*}


\subsection*{(b) Find the transient and steady state currents)}

\textbf{Solution:} We will start by finding the transient current

\begin{align*}
I_{transient} &= -1.1e^{-40t} \\
\lim_{t \to \infty} -1.1e^{-40t} &= 0 \\
I_{transient} &= 0
\end{align*}

Next we will find the steady state current

\begin{align*}
\lim_{t \to \infty} 1.1 + ce^{-40t} &= 1.1 \\
I_{steady} &= 1.1
\end{align*}

\subsection*{(c) Find the time required for the current to reach $0.6$ amps}

\textbf{Solution:} Set I = 0.6 and solve for t

\begin{align*}
0.6 &= 1.1(1 - e^{-40t}) \\
\frac{0.6}{111} &= 1 - e^{-40t} \\
e^{-40t} &= \frac{0.5}{1.1} \\
-40t &= \ln(\frac{0.5}{1.1}) \\
t &= \frac{\ln(\frac{0.5}{1.1})}{-40}
\end{align*}

\section*{Problem 8}
\textbf{Problem Statement:} Solve the differential equation $(x+1)\frac{dy}{x}+y = \ln(t)$

\textbf{Solution:} We will solve using the integrating factor method
Rewriting the equation:
\[
\frac{dy}{dt} + \frac{y}{t+1} = \frac{lnt}{t+1}
\]

Set right side equal to zero
\[
\frac{dy}{dt} + \frac{y}{t+1} = 0
\]

Solve for y
\begin{align*}
\frac{dy}{dt} &= -\frac{y}{t+1} \\
\frac{dy}{y} &= -\frac{dt}{t+1} \\
\end{align*}

Integrate both sides
\begin{align*}
\int \frac{1}{y} dy &= -\frac{1}{t+1} dt \\
\ln|y| &= -ln|t+1| + c \\
y &= e^{-\ln|t+1| + c} \\
y&= \frac{c}{t+1}
\end{align*}

Solve for integrating factor $\mu$
\begin{align*}
\mu &= \frac{1}{y_{G,H}} \\
\mu &= t+1
\end{align*}


Multiply orignial equation by $\mu$
\begin{align*}
\mu \frac{dy}{dt} + \mu \frac{y}{t+1} &= \mu \frac{lnt}{t+1} \\
D[(t+1)y] &= \frac{\ln(t)}{t+1}(t+1) \\
(t+1)y &= \int \ln(t) \\
(t+1)y &= t\ln(t) - t + c \\
y &= \frac{t\ln(t) - t + c}{t+1}
\end{align*}

\section*{Problem 9}

\textbf{Problem Statement:} Use the Euler-Lagrange Two-Stage Method to sole the IVP $\frac{dy}{dt} + 2ty = t^3, \quad y(1) = 1$

\textbf{Solution:} We will start by finding the general solution to the Homogeneous ODE

\begin{align*}
\frac{dy}{dt} + 2ty &= 0 \\
\frac{dy}{y} &= -2tdt \\
\ln|y| &= -t^2 + c \\
y &= ce^{-t^2}
\end{align*}

We will now substitute a fucntion $v(t)$ for the constant $c$:

\begin{align*}
y = v(t)e^{-t^2}
\end{align*}

We will now determine the function $v(t)$ by substituting $y$ into the oringinal Non-Homogeneous ODE

\begin{align*}
\frac{dy}{dt} + 2ty &= t^3 \\
\frac{d(v(t)e^{-t^2})}{dt} + 2t(v(t)e^{-t^2}) &= t^3 \\
\frac{dv}{dt}e^{-t^2} - 2te^{-t^2}v + 2te^{-t^2}v &= t^3 \\
\frac{dv}{dt}e^{-t^2} &= t^3 \\
\frac{dv}{dt} &= t^3e^{t^2} \\
\end{align*}

Integrating both sides using $u = t^2$,

\begin{align*}
v &= \frac{1}{2}\int ue^{u}du \\
v &= \frac{1}{2}(t^2 - 1) + Ce^{-t^2}
\end{align*}

Now we will substitute $v$ back into the equation for $y$

\begin{align*}
y &= (\frac{1}{2}(t^2 - 1) + Ce^{-t^2})e^{-t^2} \\
y &= \frac{1}{2}(t^2 - 1)e^{-t^2} + Ce^{-2t^2}
\end{align*}

Using the superposition principal, $y_{G,NH} = y_{G,H} + y_{P,NH}$, we will solve for the general solution to the Non-Homogeneous ODE

\begin{align*}
   y_G,NH &= \frac{1}{2}(t^2 - 1) + ce^{-2t^2} + ce^{-t^2}
   y_G,NH &= \frac{1}{2}(t^2 - 1) + ce^{-2t^2}
\end{align*}

Solve the IVP $y(1) = 1$

\begin{align*}
    1 &= \frac{1}{2}(1 - 1) + ce^{-1^2} \\
    1 &= c \cdot e^{1} \\
    c &= e^1
\end{align*}

Therefore, the solution to the IVP is

\begin{align*}
    y &= \frac{1}{2}(t^2 - 1) + e^1e^{-2t^2}
    y &= \frac{1}{2}(t^2 - 1) + e^{1-2t^2}
\end{align*}

\section*{Problem 10}

\textbf{Problem Statement:} Solve the bernoulli equation $t^2y' + 2ty = 3y^4$

\textbf{Solution:} We will use the substitution $v = y^{1-4}$
\begin{align*}
    v &= y^{1-4} \\
    v &= y^{-3} \\
    y^3 &= v^{-1} \\
    y &= v^{-1/3}
\end{align*}

Now we will find the derivative of $y$

\begin{align*}
    y &= v^{-1/3} \\
    \frac{dy}{dt} &= -\frac{1}{3}v^{-4/3}\frac{dv}{dt}
\end{align*}

Now we will substitute $y$ and $\frac{dy}{dt}$ into the Bernoulli equation

\begin{align*}
    t^2y' + 2ty = 3y^4
    y' + \frac{2y}{t} &= \frac{3}{t^2}y^4 \\
    -\frac{1}{3}v^{-4/3}\frac{dv}{dt} + \frac{2}{t}v^{-1/3} &= \frac{3}{t^2}v^{-4/3} \\
    -\frac{1}{3}\frac{dv}{dt} + \frac{2}{t}v &= \frac{3}{t^2}v \\
    \frac{dv}{dt} - \frac{6}{t}v &= -\frac{9}{t^2}v
\end{align*}

Now we will solve the ODE using the integrating factor method.

\begin{align*}
    \mu &= e^{\int -\frac{6}{t}dt} \\
    \mu &= e^{-6\ln|t|} \\
    \mu &= e^{\ln|t^{-6}|} \\
    \mu &= t^{-6}
\end{align*}

Multiplying the ODE by $\mu$

\begin{align*}
    \mu \frac{dv}{dt} - \frac{d\mu}{dt}v &= \frac{-9}{t^2} \mu \\
    D[\mu v] &= \frac{-9}{t^2} \mu \\
    t^{-6}v &= \int -9t^{-8}v \\
    t^{-6}v &= -\frac{9}{-7}t^{-7}v + c \\
    v &= \frac{9}{7}t^{-1} + ct^6 \\
\end{align*}

Now we will substitute $y$ back into the equation for $v$

\begin{align*}
    v &= y^3 \\
    y^3 &= \frac{9}{7}t^{-1} + ct^6 \\
    y &= (\frac{9}{7}t^{-1}+ ct^6)^{-1/3}
\end{align*}



\end{document}